cklr/Inject.v
@@ -18,23 +18,25 @@ Record inj_world :=
   }.
 
 Variant inj_incr: relation inj_world :=
-  inj_incr_intro f f' nb1 nb2:
+  inj_incr_intro f f' nb1 nb2 nb1' nb2':
     inject_incr f f' ->
     (forall b1 b2 delta, f b1 = None -> f' b1 = Some (b2, delta) ->
      Pos.le nb1 b1 /\ Pos.le nb2 b2) ->
-    inj_incr (injw f nb1 nb2) (injw f' nb1 nb2).
+    Pos.le nb1 nb1' ->
+    Pos.le nb2 nb2' ->
+    inj_incr (injw f nb1 nb2) (injw f' nb1' nb2').
 
 Variant inj_stbls: klr inj_world Genv.symtbl Genv.symtbl :=
-  inj_stbls_intro f se1 se2:
+  inj_stbls_intro f nb1 nb2 se1 se2:
     Genv.match_stbls f se1 se2 ->
-    inj_stbls (injw f (Genv.genv_next se1) (Genv.genv_next se2)) se1 se2.
+    Pos.le (Genv.genv_next se1) nb1 ->
+    Pos.le (Genv.genv_next se2) nb2 ->
+    inj_stbls (injw f nb1 nb2) se1 se2.
 
 Variant inj_mem: klr inj_world mem mem :=
-  inj_mem_intro f m1 m2 nb1 nb2:
+  inj_mem_intro f m1 m2:
     Mem.inject f m1 m2 ->
-    Pos.le nb1 (Mem.nextblock m1) ->
-    Pos.le nb2 (Mem.nextblock m2) ->
-    inj_mem (injw f nb1 nb2) m1 m2.
+    inj_mem (injw f (Mem.nextblock m1) (Mem.nextblock m2)) m1 m2.
 
 (** ** Properties *)
 
@@ -53,13 +55,14 @@ Global Instance inj_incr_preo:
 Proof.
   split.
   - intros [f nb1 nb2].
-    constructor; auto using inject_incr_refl.
+    constructor; auto using inject_incr_refl, Pos.le_refl.
     congruence.
   - intros w w' w'' H H'. destruct H. inv H'.
-    constructor; eauto using inject_incr_trans.
+    constructor; eauto using inject_incr_trans, Pos.le_trans.
     intros b1 b2 delta Hb Hb''.
-    destruct (f' b1) as [[xb2 xdelta] | ] eqn:Hb'; eauto.
-    rewrite (H5 _ _ _ Hb') in Hb''. inv Hb''. eauto.
+    destruct (f' b1) as [[xb2 xdelta] | ] eqn:Hb'.
+    + rewrite (H6 _ _ _ Hb') in Hb''. inv Hb''. eauto.
+    + edestruct H7; eauto. xomega.
 Qed.
 
 Global Instance inj_stbls_subrel:
@@ -67,7 +70,9 @@ Global Instance inj_stbls_subrel:
 Proof.
   intros w w' Hw se1 se2 Hse.
   destruct Hse; inv Hw.
-  constructor. eapply Genv.match_stbls_incr; eauto.
+  constructor; try xomega.
+  eapply Genv.match_stbls_incr; eauto.
+  intros. edestruct H6; eauto. xomega.
 Qed.
 
 Instance inj_proj_incr:
@@ -87,14 +92,14 @@ Qed.
 
 Lemma inj_mem_next_l w m1 m2:
   inj_mem w m1 m2 ->
-  Pos.le (injw_next_l w) (Mem.nextblock m1).
+  injw_next_l w = Mem.nextblock m1.
 Proof.
   destruct 1; auto.
 Qed.
 
 Lemma inj_mem_next_r w m1 m2:
   inj_mem w m1 m2 ->
-  Pos.le (injw_next_r w) (Mem.nextblock m2).
+  injw_next_r w = Mem.nextblock m2.
 Proof.
   destruct 1; auto.
 Qed.
@@ -118,7 +123,7 @@ Next Obligation.
 Qed.
 
 Next Obligation.
-  destruct H. inv H0. eauto.
+  destruct H. inv H0. xomega.
 Qed.
 
 Next Obligation. (* Mem.alloc *)
@@ -128,7 +133,7 @@ Next Obligation. (* Mem.alloc *)
     as (f' & m2' & b2 & Hm2' & Hm' & Hf'1 & Hb2 & Hf'2);
     eauto using Z.le_refl.
   rewrite Hm2'.
-  exists (injw f' nb1 nb2); split; repeat rstep.
+  exists (injw f' (Mem.nextblock m1') (Mem.nextblock m2')); split; repeat rstep.
   - constructor; eauto.
     intros b1' b2' delta' Hb Hb'.
     destruct (peq b1' b1); subst.
@@ -137,6 +142,8 @@ Next Obligation. (* Mem.alloc *)
       apply Mem.alloc_result in Hm2'; subst.
       xomega.
     + specialize (Hf'2 _ n). congruence.
+    + erewrite (Mem.nextblock_alloc m1 _ _ m1'); eauto. xomega.
+    + erewrite (Mem.nextblock_alloc m2 _ _ m2'); eauto. xomega.
   - econstructor; eauto; erewrite Mem.nextblock_alloc by eauto; xomega.
   - cbn. red. auto.
 Qed.
@@ -150,7 +157,7 @@ Next Obligation. (* Mem.free *)
   replace (lo1 + delta + sz) with (lo1 + sz + delta) by xomega.
   rewrite Hm2'.
   repeat (econstructor; eauto); try congruence;
-    erewrite Mem.nextblock_free; eauto.
+    erewrite <- Mem.nextblock_free; eauto using Pos.le_refl.
 Qed.
 
 Next Obligation. (* Mem.load *)
@@ -168,7 +175,7 @@ Next Obligation. (* Mem.store *)
   edestruct Mem.store_mapped_inject as (m2' & Hm2' & Hm'); eauto.
   rewrite Hm2'.
   repeat (econstructor; eauto); try congruence;
-    erewrite Mem.nextblock_store; eauto.
+    erewrite <- Mem.nextblock_store; eauto using Pos.le_refl.
 Qed.
 
 Next Obligation. (* Mem.loadbytes *)
@@ -192,10 +199,11 @@ Next Obligation. (* Mem.storebytes *)
     }
     rewrite Hm2'.
     constructor.
-    eexists; split; repeat rstep. constructor; eauto.
-    + eapply Mem.storebytes_empty_inject; eauto.
-    + erewrite Mem.nextblock_storebytes; eauto.
-    + erewrite Mem.nextblock_storebytes; eauto.
+    eexists; split; repeat rstep.
+    erewrite <- (Mem.nextblock_storebytes m1); eauto.
+    erewrite <- (Mem.nextblock_storebytes m2); eauto.
+    constructor; eauto.
+    eapply Mem.storebytes_empty_inject; eauto.
   - assert (ptr_inject f (b1, ofs1) (b2, ofs2)) as Hptr'.
     {
       destruct Hptr as [Hptr|Hptr]; eauto.
@@ -211,7 +219,7 @@ Next Obligation. (* Mem.storebytes *)
     edestruct Mem.storebytes_mapped_inject as (m2' & Hm2' & Hm'); eauto. rauto.
     rewrite Hm2'.
     repeat (econstructor; eauto); try congruence;
-      erewrite Mem.nextblock_storebytes; eauto.
+      erewrite <- Mem.nextblock_storebytes; eauto using Pos.le_refl.
 Qed.
 
 Next Obligation. (* Mem.perm *)
@@ -449,33 +457,36 @@ Qed.
 Lemma inj_inj:
   subcklr inj (inj @ inj).
 Proof.
-  intros w se1 se2 m1 m2 Hse Hm. destruct Hm as [f m1 m2 nb1 nb2 Hm].
-  exists (injw (meminj_dom f) nb1 nb1, injw f nb1 nb2); simpl.
+  intros w se1 se2 m1 m2 Hse Hm. destruct Hm as [f m1 m2 Hm].
+  exists (injw (meminj_dom f) (Mem.nextblock m1) (Mem.nextblock m1),
+          injw f (Mem.nextblock m1) (Mem.nextblock m2)); simpl.
   repeat apply conj.
   - exists se1. split; eauto.
-    inv Hse. econstructor. eapply match_stbls_dom; eauto.
+    inv Hse. econstructor; auto. eapply match_stbls_dom; eauto.
   - exists m1; split; repeat rstep; eauto using inj_mem_intro, mem_inject_dom.
   - rewrite meminj_dom_compose.
     apply inject_incr_refl.
   - intros [w12' w23'] m1' m3' (m2' & H12' & H23') [Hw12' Hw23']. cbn in *.
-    destruct H12' as [f12' m1' m2' ? ? ? Hm12'].
-    inversion H23' as [f23' xm2' xm3' ? ? ? Hm23']. clear H23'; subst.
-    inversion Hw12' as [? ? ? ? Hf12' SEP12']. clear Hw12'; subst.
-    inversion Hw23' as [? ? ? ? Hf23' SEP23']. clear Hw23'; subst.
-    exists (injw (compose_meminj f12' f23') nb4 nb5).
+    destruct H12' as [f12' m1' m2' Hm12'].
+    inversion H23' as [f23' xm2' xm3' Hm23']. clear H23'; subst.
+    inversion Hw12' as [? ? ? ? ? ? Hf12' SEP12']. clear Hw12'; subst.
+    inversion Hw23' as [? ? ? ? ? ? Hf23' SEP23']. clear Hw23'; subst.
+    eexists (injw (compose_meminj f12' f23') _ _).
     repeat apply conj.
     + constructor; auto. eapply Mem.inject_compose; eauto.
-    + constructor.
+    + constructor; auto.
       * rewrite <- (meminj_dom_compose f). rauto.
       * intros b1 b2 delta Hb Hb'. unfold compose_meminj in Hb'.
         destruct (f12' b1) as [[bi delta12] | ] eqn:Hb1; try discriminate.
         destruct (f23' bi) as [[xb2 delta23] | ] eqn:Hb2; try discriminate.
-        inv Hb'. inv Hse.
+        inv Hb'.
         edestruct SEP12'; eauto. unfold meminj_dom. rewrite Hb. auto.
-        destruct (f bi) as [[xb2 xdelta23] | ] eqn:Hbi.
-        -- rewrite (Hf23' _ _ _ Hbi) in Hb2. inv Hb2.
-           rewrite <- (Genv.mge_separated H10 _ Hbi). auto.
-        -- edestruct (SEP23' bi b2); eauto. 
+        destruct (f bi) as [[? ?] | ] eqn:Hfbi.
+        {
+          eapply Mem.valid_block_inject_1 in Hfbi; eauto.
+          red in Hfbi. xomega.
+        }
+        edestruct SEP23'; eauto. 
     + cbn. rstep; auto.
 Qed.
 
@@ -499,6 +510,6 @@ Proof.
     + constructor; eauto.
     + constructor; eauto.
       constructor; eauto.
-    + intros r1 r2 (w' & Hw' & Hr). inv Hw'. inv Hr. inv H7. cbn in *.
+    + intros r1 r2 (w' & Hw' & Hr). inv Hw'. inv Hr. inv H3. cbn in *.
       eexists; eauto. constructor; eauto.
 Qed.
